Logic/Modal/Normal/ModalCompanion.lean
@@ -35,10 +35,10 @@ end GTranslation
 lemma intAxiom4 {p : Intuitionistic.Formula α} : ∅ ⊢ᴹ[𝐊𝟒]! pᵍ ⟶ □pᵍ := by
   induction p using Intuitionistic.Formula.rec' with
   | hatom => simp; apply axiom4!;
-  | hfalsum => apply dtr!; apply efq'!; apply axm!; simp;
+  | hfalsum => apply dtr'!; apply efq'!; apply axm!; simp;
   | himp => simp; apply axiom4!;
   | hand p q ihp ihq =>
-    apply dtr!;
+    apply dtr'!;
     have : {pᵍ ⋏ qᵍ} ⊢ᴹ[𝐊𝟒]! pᵍ ⋏ qᵍ := axm! (by simp);
     have : {pᵍ ⋏ qᵍ} ⊢ᴹ[𝐊𝟒]! □pᵍ := by simpa using modus_ponens'! ihp $ conj₁'! (by assumption);
     have : {pᵍ ⋏ qᵍ} ⊢ᴹ[𝐊𝟒]! □qᵍ := by simpa using modus_ponens'! ihq $ conj₂'! (by assumption);
@@ -46,9 +46,9 @@ lemma intAxiom4 {p : Intuitionistic.Formula α} : ∅ ⊢ᴹ[𝐊𝟒]! pᵍ ⟶
     have : {pᵍ ⋏ qᵍ} ⊢ᴹ[𝐊𝟒]! □(pᵍ ⋏  qᵍ) := collect_box_conj'! (by assumption);
     simpa;
   | hor p q ihp ihq =>
-    apply dtr!;
-    have hp : ∅ ⊢ᴹ[𝐊𝟒]! pᵍ ⟶ □(pᵍ ⋎ qᵍ) := dtr! $ collect_box_disj'! $ disj₁'! $ by simpa using dtl! ihp;
-    have hq : ∅ ⊢ᴹ[𝐊𝟒]! qᵍ ⟶ □(pᵍ ⋎ qᵍ) := dtr! $ collect_box_disj'! $ disj₂'! $ by simpa using dtl! ihq;
+    apply dtr'!;
+    have hp : ∅ ⊢ᴹ[𝐊𝟒]! pᵍ ⟶ □(pᵍ ⋎ qᵍ) := dtr'! $ collect_box_disj'! $ disj₁'! $ by simpa using dtl'! ihp;
+    have hq : ∅ ⊢ᴹ[𝐊𝟒]! qᵍ ⟶ □(pᵍ ⋎ qᵍ) := dtr'! $ collect_box_disj'! $ disj₂'! $ by simpa using dtl'! ihq;
     have h : {pᵍ ⋎ qᵍ} ⊢ᴹ[𝐊𝟒]! pᵍ ⋎ qᵍ := axm! (by simp);
     simpa using disj₃'! (weakening! (by simp) hp) (weakening! (by simp) hq) h;
 
